compiler/src/Op.v
@@ -1,49 +1,23 @@
-Require Import compiler.util.Common.
 Require Import riscv.Utility.
 
+Module bopname.
+  Inductive bopname := add | sub | mul | and | or | xor | sru | slu | srs | lts | ltu | eq.
+End bopname.
 
-Inductive binop: Set := OPlus | OMinus | OTimes | OEq | OLt | OAnd.
+Notation bopname := bopname.bopname.
 
-Definition eval_binop{t: Set}{MW: MachineWidth t}(op: binop)(v1 v2: t): t :=
+Definition eval_binop{t: Set}{MW: MachineWidth t}(op: bopname)(v1 v2: t): t :=
   match op with
-  | OPlus => add v1 v2
-  | OMinus => sub v1 v2
-  | OTimes => mul v1 v2
-  | OEq => if reg_eqb v1 v2 then ZToReg 1 else (ZToReg 0)
-  | OLt => if ltu v1 v2 then ZToReg 1 else (ZToReg 0)
-  | OAnd => and v1 v2
+  | bopname.add => add v1 v2
+  | bopname.sub => sub v1 v2
+  | bopname.mul => mul v1 v2
+  | bopname.and => and v1 v2
+  | bopname.or  => or  v1 v2
+  | bopname.xor => xor v1 v2
+  | bopname.sru => srl v1 (regToShamt v2)
+  | bopname.slu => sll v1 (regToShamt v2)
+  | bopname.srs => sra v1 (regToShamt v2)
+  | bopname.ltu => if ltu v1 v2              then ZToReg 1 else ZToReg 0
+  | bopname.lts => if signed_less_than v1 v2 then ZToReg 1 else ZToReg 0
+  | bopname.eq  => if reg_eqb v1 v2          then ZToReg 1 else ZToReg 0
   end.
-
-Definition eval_binop_word{w: Z}(op: binop)(v1 v2: word w): word w :=
-  match op with
-  | OPlus => wadd v1 v2
-  | OMinus => wsub v1 v2
-  | OTimes => wmul v1 v2
-  | OEq => if weqb  v1 v2 then ZToWord w 1 else ZToWord w 0
-  | OLt => if wultb v1 v2 then ZToWord w 1 else ZToWord w 0
-  | OAnd => wand v1 v2
-  end.
-
-Definition eval_binop_nat(op: binop)(v1 v2: nat): nat :=
-  match op with
-  | OPlus => v1 + v2
-  | OMinus => v1 - v2
-  | OTimes => v1 * v2
-  | OEq => if Nat.eq_dec v1 v2 then 1 else 0
-  | OLt => if Compare_dec.lt_dec v1 v2 then 1 else 0
-  | OAnd => Z.to_nat (Z.land (Z.of_nat v1) (Z.of_nat v2))
-  end.
-
-Definition eval_binop_Z_unbounded(op: binop)(v1 v2: Z): Z :=
-  match op with
-  | OPlus => v1 + v2
-  | OMinus => v1 - v2
-  | OTimes => v1 * v2
-  | OEq => if dec (v1 = v2) then 1 else 0
-  | OLt => if dec (v1 < v2)%Z then 1 else 0
-  | OAnd => (Z.land v1 v2)
-  end.
-
-Definition eval_binop_Z_bounded(w: nat)(op: binop)(v1 v2: Z): Z :=
-  let mask := Z.ones (Z.of_nat w) in
-  Z.land mask (eval_binop_Z_unbounded op v1 v2).
