compiler/src/NamesInstance.v
@@ -6,5 +6,5 @@ Instance Names: bedrock2.Syntax.parameters := {|
   bedrock2.Syntax.varname := Z;
   bedrock2.Syntax.funname := Z;
   bedrock2.Syntax.actname := Empty_set;
-  bedrock2.Syntax.bopname := binop;
+  bedrock2.Syntax.bopname := bopname;
 |}.
