compiler/src/examples/highlevel/FuncMut.v
@@ -2,7 +2,21 @@ Require Import Coq.Lists.List.
 Import ListNotations.
 Require Import compiler.Decidable.
 Require Import riscv.util.Monads.
-Require Import compiler.Op.
+Require Import compiler.util.Common.
+
+Inductive binop: Set := OPlus | OMinus | OTimes | OEq | OLt | OAnd.
+
+Definition eval_binop_nat(op: binop)(v1 v2: nat): nat :=
+  match op with
+  | OPlus => v1 + v2
+  | OMinus => v1 - v2
+  | OTimes => v1 * v2
+  | OEq => if Nat.eq_dec v1 v2 then 1 else 0
+  | OLt => if Compare_dec.lt_dec v1 v2 then 1 else 0
+  | OAnd => Z.to_nat (Z.land (Z.of_nat v1) (Z.of_nat v2))
+  end.
+
+
 
 (* A mix between imperative and functional:
    It has expressions and lets, but mutable arrays.
